CollapsingTowers/TwoLevelMut/OperationalSemantics/Congruence.lean
@@ -1,5 +1,45 @@
 import CollapsingTowers.TwoLevelMut.OperationalSemantics.SmallStep
 
+lemma step_grounded.congruence_under_ctx𝔹 : ∀ B σ₀ σ₁ e₀ e₁, ctx𝔹 B → grounded e₀ → (⟨σ₀, e₀⟩ ⇝ ⟨σ₁, e₁⟩) → (⟨σ₀, B⟦e₀⟧⟩ ⇝ ⟨σ₁, B⟦e₁⟧⟩) :=
+  by
+  intros B σ₀ σ₁ e₀ e₁ HB HG Hstep
+  cases Hstep
+  case pure M _ _ HM Hlc Hhead =>
+    repeat rw [ctx_comp B M]
+    apply step_lvl.pure
+    apply ctx𝕄.cons𝔹; apply HB; apply HM
+    apply Hlc; apply Hhead
+  case mutable M _ _ HM Hlc Hmut =>
+    repeat rw [ctx_comp B M]
+    apply step_lvl.mutable
+    apply ctx𝕄.cons𝔹; apply HB; apply HM
+    apply Hlc; apply Hmut
+  case reflect M E _ HP HE _ =>
+    have HM := rewrite.ctxℙ_ctx𝕄 _ _ HP
+    have HG := grounded.decompose_ctx𝕄 _ _ _ HM HG
+    have HG := grounded.decompose_ctx𝔼 _ _ HE HG
+    simp at HG
+
+lemma stepn_grounded.congruence_under_ctx𝔹 : ∀ B σ₀ σ₁ e₀ e₁, ctx𝔹 B → grounded e₀ → (⟨σ₀, e₀⟩ ⇝* ⟨σ₁, e₁⟩) → (⟨σ₀, B⟦e₀⟧⟩ ⇝* ⟨σ₁, B⟦e₁⟧⟩) :=
+  by
+  intros B σ₀ σ₂ e₀ e₂ HB HG Hstepn
+  generalize HEq₀ : (σ₀, e₀) = st₀
+  generalize HEq₁ : (σ₂, e₂) = st₂
+  rw [HEq₀, HEq₁] at Hstepn
+  induction Hstepn generalizing σ₀ e₀
+  case refl st₁ =>
+    rcases st₁ with ⟨σ₁, e₁⟩
+    simp at HEq₀ HEq₁
+    simp [HEq₀, HEq₁]
+    apply stepn.refl
+  case multi st₀ st₁ st₂ Hstep Hstepn IH =>
+    rcases st₁ with ⟨σ₁, e₁⟩
+    rw [← HEq₀] at Hstep
+    apply stepn.multi
+    apply step_grounded.congruence_under_ctx𝔹
+    apply HB; apply HG; apply Hstep
+    apply IH _ _ (grounded.under_step _ _ _ _ Hstep HG) rfl HEq₁
+
 lemma step.congruence_under_ctx𝔹 :
   ∀ lvl B σ₀ σ₁ e₀ e₁,
     ctx𝔹 B →
